Add contract monads
- Add a monad typeclass and switch option monad to an instance of this
- Add monads for contract functions, allowing access to blockchain state
  and a nicer interface for rejecting/accepting

execution/theories/Monads.v
@@ -1,21 +1,54 @@
-(* This file defines some helpful notations for the option monad. *)
+(* This file defines some helpful notations for monads. *)
 
-Definition option_bind {A B : Type} (v : option A) (f : A -> option B) : option B :=
-  match v with
-  | Some val => f val
-  | None => None
-  end.
+Class Monad (m : Type -> Type) : Type :=
+build_monad {
+  ret : forall {t}, t -> m t;
+  bind : forall {t u}, m t -> (t -> m u) -> m u
+}.
 
-Notation "c >>= f" := (option_bind c f) (at level 50, left associativity).
-Notation "f =<< c" := (option_bind c f) (at level 51, right associativity).
+Notation "c >>= f" := (bind c f) (at level 50, left associativity).
+Notation "f =<< c" := (bind c f) (at level 51, right associativity).
 
 Notation "'do' x <- c1 ; c2" :=
-  (option_bind c1 (fun x => c2))
+  (bind c1 (fun x => c2))
     (at level 60, c1 at next level, right associativity).
 
 Notation "'do' ' pat <- c1 ; c2" :=
-  (option_bind c1 (fun x => match x with pat => c2 end))
+  (bind c1 (fun x => match x with pat => c2 end))
     (at level 60, pat pattern, c1 at next level, right associativity).
 
 Notation "'do' e1 ; e2" := (do _ <- e1 ; e2)
   (at level 60, right associativity).
+
+Class MonadLaws {m : Type -> Type} (mon : Monad m) :=
+build_monad_laws {
+  bind_of_return :
+    forall (T : Type) (t : T) (U : Type) (f : T -> m U),
+      (ret t >>= f) = f t;
+  return_of_bind :
+    forall (T : Type) (t : m T),
+      (t >>= @ret m mon T) = t;
+  bind_assoc :
+    forall (T U V : Type) (t : m T) (f : T -> m U) (g : U -> m V),
+      (t >>= f) >>= g = t >>= (fun t => f t >>= g);
+}.
+
+Class MonadTrans (m : Type -> Type) (mt : Type -> Type) : Type :=
+  { lift : forall {t}, mt t -> m t }.
+
+Global Instance option_monad : Monad option :=
+  {| ret _ t := Some t;
+     bind _ _ v f := match v with
+                 | Some val => f val
+                 | None => None
+                 end |}.
+
+Global Instance option_monad_laws : MonadLaws option_monad.
+Proof.
+  constructor.
+  - auto.
+  - intros; cbn.
+    destruct t; auto.
+  - intros; cbn.
+    destruct t; auto.
+Qed.
